\begin{myTheorem}[Recursion]
The integrals in \eqref{eq:family Y} can be generated using
  % % % EQUATION
\begin{equation}
  \begin{split}
    \mathcal{Y}_{0}(b)   &= \cost \\
    \mathcal{Y}_{n+2}(b) &= \paren{\paren{n + 2} \frac{b^{2}}{\cost} \mathcal{Y}_{n}(b) + 1} \frac{\cost}{n + 3}, \qquad n = 2, 4, 6, \dots.
  \end{split}
\label{eq:recursion Y}
\end{equation}
  % % % EQUATION
\end{myTheorem}  %  -  -  -  -  -  -  -  -  -  -  -  -  -  -  -  -
\begin{proof}  %  +  +  +  +  +  +  +  +  +  +  +  +  +  +  +  +
The base case $\mathcal{Y}_{0}(b)$ is trivial; consider $n=2,4,\dots$. Attack the integral
  % % % EQUATION
  \begin{equation}
    \mathcal{Y}_{n}(b) = \int_{0}^{\cost} \paren{ \xpbs }^{n} dx_{1}
  \end{equation}
  % % %
using integration by parts, $\int udv = uv - \int vdu$, where 
  % - -  e q u a t i o n
  \begin{equation}
    u = \paren{ \xpbs }^{n}, \quad dv = dx_{1}
  \end{equation}
  % - -
which leads to the identity
  % % % EQUATION
  \begin{equation}
    \int_{0}^{\cost} \paren{ \xpbs }^{n} dx_{1} = \cost - n 
    \int_{0}^{\cost} x_{1}^{2} \paren{ \xpbs }^{n-2} dx_{1}.
  \end{equation}
  % % %
Let the multiplicative factor $x_{1}^{2} = x_{1}^{2} + b^{2} - b^{2}$ and shift the index $n$ up by 2 to recover \eqref{eq:recursion Y}.
\end{proof}

\endinput %-------------------------------